

Ch 6.1, 6.2, 6.5: LU Factorization, part 1 (basics)

Saturday, December 6, 2025

7:13 PM

Should be a review of what students saw in APPM 3310

LU factorization is how we actually do Gaussian Elimination on a computer

This is ch. 6.5 in Burden and Faires on Matrix Factorization

LU is an example of a matrix factorization

means writing your matrix "A" as the product of other matrices which have special properties

Ex of matrix factorizations

covered in our class

LU ch. 4 $A = L \cdot U$ L is Lower triangular, U is Upper triangular

Eigenvalue ch. 9 $A = V D V^{-1}$ V is invertible, D is diagonal (only for square matrices)

"SVD" end of ch. 9. We don't normally cover, but the factorization is super useful
Singular Value $A = V \Sigma U^T$ V, U are orthogonal ($V^T V = I \dots$), Σ is a diagonal matrix w/ non-zero entries

QR $A = Q R$ Q is orthogonal, R is upper triangular (like Gram-Schmidt)

Schur, Polar not as common (though Schur is a useful intermediate step for eigenvalues)

LDL^T , Cholesky variants of LU that we'll talk about briefly

LU decomposition to solve a linear system of equations

want to solve $A \vec{x} = \vec{b}$, suppose we can write $A = L U$
 $n \times n$ (square) lower triag. upper triag.

so solve $L U \vec{x} = \vec{b}$
let $\vec{y} = U \vec{x}$

$$\boxed{A} = \boxed{L} \cdot \boxed{U}$$

① Solve $L \vec{y} = \vec{b}$

This is "easy" ($O(n^2)$ flops not $O(n^3)$) since L is Lower Triangular

"Forward Substitution"

$$\begin{matrix} 3 \times 3 \\ \text{example:} \end{matrix} \begin{bmatrix} L_{11} & 0 & 0 \\ L_{21} & L_{22} & 0 \\ L_{31} & L_{32} & L_{33} \end{bmatrix} \begin{bmatrix} y_1 \\ y_2 \\ y_3 \end{bmatrix} = \begin{bmatrix} b_1 \\ b_2 \\ b_3 \end{bmatrix}$$

$$1) L_{11} y_1 = b_1 \text{ so } y_1 = b_1 / L_{11}$$

$$2) L_{21} y_1 + L_{22} y_2 = b_2 \text{ so } y_2 = (b_2 - L_{21} y_1) / L_{22}$$

$$3) L_{31} y_1 + L_{32} y_2 + L_{33} y_3 = b_3$$

② Solve $U\vec{x} = \vec{y}$

Also "easy" ($O(n^2)$) since U is upper triangular

"Back substitution"

$$\begin{bmatrix} u_{11} & u_{12} & u_{13} \\ 0 & u_{22} & u_{23} \\ 0 & 0 & u_{33} \end{bmatrix} \begin{bmatrix} x_1 \\ x_2 \\ x_3 \end{bmatrix} = \begin{bmatrix} y_1 \\ y_2 \\ y_3 \end{bmatrix}$$

3) $u_{33} x_3 = y_3$

2) $u_{22} x_2 + u_{23} x_3 = y_2$

1) $u_{11} x_1 + u_{12} x_2 + u_{13} x_3 = y_1$

★ TRIANGULAR SYSTEMS OF EQUATIONS ARE EASY TO SOLVE
IF YOU SOLVE THEM IN THE RIGHT ORDER

Interlude: block matrix multiplication

Ex. $\begin{bmatrix} \begin{matrix} \text{2} \\ \text{4} \\ \text{2} \end{matrix} \begin{bmatrix} \text{B} & \text{C} \\ \text{D} & \text{E} \end{bmatrix} \end{bmatrix} \cdot \begin{bmatrix} \text{F} \\ \text{G} \end{bmatrix} = \begin{bmatrix} \text{BF} + \text{CG} \\ \text{DF} + \text{EG} \end{bmatrix}$

Any size blocks work (as long as they're all compatible)

So, if A is square, and we want to keep the 1st block of $A\vec{x}$ the same as \vec{x} , meaning $F = BF + CG$ then choose $B = I$
 $C = 0$

Finding the LU decomposition

We'll do Gaussian elimination, and it'll cost $O(n^3)$ flops, so this is the expensive part

"Gaussian Elimination = LU"

$$A\vec{x} = \vec{b} \quad \begin{bmatrix} a_{11} & a_{12} & a_{13} \\ a_{21} & a_{22} & a_{23} \\ a_{31} & a_{32} & a_{33} \end{bmatrix} \begin{bmatrix} b_1 \\ b_2 \\ b_3 \end{bmatrix}$$

E_1 (row 1), E_2 (row 2), E_3 (row 3)

$$E_2 \leftarrow E_2 - \alpha_{21}/a_{11} \cdot E_1$$

$$E_3 \leftarrow E_3 - \alpha_{31}/a_{11} \cdot E_1$$

$E_i = i^{\text{th}}$ row

to get we "zeroed out" 1st column

$$\begin{bmatrix} a_{11} & a_{12} & a_{13} & | & b_1 \\ 0 & \text{something} & \text{something} & | & \text{something} \\ 0 & \text{something} & \text{something} & | & \text{something} \end{bmatrix}$$

just means "something"

Connect this step to matrix multiplication

$$\begin{bmatrix} 1 & 0 & 0 \\ -\alpha_2 & 1 & 0 \\ -\alpha_3 & 0 & 1 \end{bmatrix} \cdot \begin{bmatrix} a_1 \\ a_2 \\ a_3 \end{bmatrix} = \begin{bmatrix} a_1 \\ -\alpha_2 a_1 + a_2 \\ -\alpha_3 a_1 + a_3 \end{bmatrix}$$

Recall
 $A \cdot [\vec{y}_1, \vec{y}_2, \vec{y}_3]$
 $= [A\vec{y}_1, A\vec{y}_2, A\vec{y}_3]$

$$\stackrel{<0}{\underbrace{\begin{bmatrix} 1 & 0 & 0 \\ -\alpha_2 & 1 & 0 \\ -\alpha_3 & 0 & 1 \end{bmatrix}}_{M^{(1)}}} \cdot \begin{bmatrix} a_{11} & a_{12} & a_{13} \\ a_{21} & a_{22} & a_{23} \\ a_{31} & a_{32} & a_{33} \end{bmatrix} = \begin{bmatrix} a_{11} & a_{12} & a_{13} \\ 0 & \sim & \sim \\ 0 & \sim & \sim \end{bmatrix}$$

So that 1st step of Gaussian Elimination was equivalent to

$$M^{(1)} A \vec{x} = M^{(1)} \vec{b}$$

Now we do more steps, but ignore 1st row

$$\text{so } M^{(2)} = \begin{bmatrix} \boxed{1} & \boxed{0} & \boxed{0} \\ 0 & \boxed{1} & 0 \\ 0 & \sim & \boxed{1} \end{bmatrix}$$

this has the block structure we just talked about in the interlude

$$M^{(2)} M^{(1)} A \vec{x} = M^{(2)} M^{(1)} \vec{b}$$

For a $n \times n$ matrix, end up with

$$\underbrace{M^{(n-1)} M^{(n-2)} \dots M^{(1)}}_{\tilde{L}} A \vec{x} = M^{(n-1)} M^{(n-2)} \dots M^{(1)} \vec{b}$$

$\rightarrow U$

We know that via Gaussian elimination, we get

\sim just means some number I don't want to give a variable name

$$\left[\begin{array}{ccc|c} \sim & \sim & \sim & \sim \\ 0 & \sim & \sim & \sim \\ 0 & 0 & \sim & \sim \end{array} \right]$$

upper triangular U

$\tilde{L} \vec{b}$

i.e.

$$\tilde{L} A = U, \text{ so } A = L U \text{ if } L := \tilde{L}^{-1}$$

U is upper triangular (via design of Gaussian elimination)

but is L really Lower triangular?

1) note $M^{(i)}$ are lower triangular. Is the product of two lower triangular matrices also lower triangular?

Yes!

$$(L^{(1)} L^{(2)})_{ij} = \boxed{0} = 0 \text{ if } j > i$$

So, $M^{(3)} M^{(2)} M^{(1)}$ is also lower triangular!

etc. $\Rightarrow \tilde{L} = M^{(n-1)} M^{(n-2)} \dots M^{(2)} M^{(1)}$ is lower triangular

2) if \tilde{L} is lower triangular, is its inverse $L := \tilde{L}^{-1}$ also lower triangular?

yes! the inverse is the solution X to the equation $\tilde{L} X = I$

then the j^{th} column of X (i.e., of L) solves

$$\begin{bmatrix} \sim & 0 & 0 & \dots & 0 \\ \sim & \sim & 0 & & \\ \sim & \sim & \sim & & \\ \vdots & & & \ddots & \\ \sim & \sim & & & \sim \end{bmatrix} \begin{bmatrix} x_{1j} \\ x_{2j} \\ \vdots \\ x_{nj} \end{bmatrix} = \begin{bmatrix} 0 \\ 0 \\ \vdots \\ 1 \\ \vdots \\ 0 \end{bmatrix}$$

$\underbrace{\quad}_{e_j}$ $\leftarrow j^{\text{th}} \text{ spot}$

So by forward substitution,

$$L_{11} x_{1j} = 0 \Rightarrow x_{1j} = 0$$

etc.

until we get to x_{jj}

So...

Gaussian elimination gave us $\tilde{L} A = U$ which we

can use to solve $(\tilde{L} A \vec{x} = U \vec{x}) = \tilde{L} \vec{b}$ (i.e. multiply $A \vec{x} = \vec{b}$ by \tilde{L} on the left)

or, similarly, $L := \tilde{L}^{-1}$

$A = L U$ and solve as we did earlier